---
title     : "The call-by-name reduction strategy"
layout    : page
prev      : /Confluence/
permalink : /CallByName/
next      : /Denotational/
---

\begin{code}
module plfa.CallByName where
\end{code}

## Imports

\begin{code}
open import plfa.Untyped
  using (Context; _⊢_; _∋_; ★; ∅; _,_; Z; S_; `_; ƛ_; _·_; subst; subst-zero;
         exts; rename)
open import plfa.LambdaReduction
  using (β; _—↠_; _—→⟨_⟩_; _[]; —↠-trans; appL-cong)
open import plfa.Soundness
  using (Subst)
open import plfa.Substitution
  using (ids; rename-subst; sub-id; sub-sub)
import Relation.Binary.PropositionalEquality as Eq
open Eq using (_≡_; _≢_; refl; trans; sym; cong; cong₂; cong-app)
open Eq.≡-Reasoning using (begin_; _≡⟨⟩_; _≡⟨_⟩_; _∎)

open import Data.Product using (_×_; Σ; Σ-syntax; ∃; ∃-syntax; proj₁; proj₂)
  renaming (_,_ to ⟨_,_⟩)
open import Function using (_∘_)
\end{code}

## Call-by-name evaluation strategy for the lambda calculus

The call-by-name strategy is a deterministic method for computing the
result of a program in the lambda calculus. We shall prove that the
call-by-name strategy produces a result if and only if full beta
reduction can reduce the program to a lambda abstraction.

We shall present the call-by-name strategy using a format that is
straightforward to implement: as a big-step semantics that uses
environments to handle variables. The environment maps each variable
to a closure, that is, to a term paired with its
environment. (Environments and closures are mutually recursive.) We
define environments and closures as follows.

\begin{code}
ClosEnv : Context → Set

data Clos : Set where
  clos : ∀{Γ} → (M : Γ ⊢ ★) → ClosEnv Γ → Clos

ClosEnv Γ = ∀ (x : Γ ∋ ★) → Clos
\end{code}

As usual, we have the empty environment, and we can extend an
environment.
\begin{code}
∅' : ClosEnv ∅
∅' ()

_,'_ : ∀ {Γ} → ClosEnv Γ → Clos → ClosEnv (Γ , ★)
(γ ,' c) Z = c
(γ ,' c) (S x) = γ x
\end{code}

The following is the big-step semantics for call-by-name evaluation,
which we describe below.

\begin{code}
data _⊢_⇓_ : ∀{Γ} → ClosEnv Γ → (Γ ⊢ ★) → Clos → Set where

  ⇓-var : ∀{Γ}{γ : ClosEnv Γ}{x : Γ ∋ ★}{Δ}{δ : ClosEnv Δ}{M : Δ ⊢ ★}{c}
        → γ x ≡ clos M δ
        → δ ⊢ M ⇓ c
          -----------
        → γ ⊢ ` x ⇓ c

  ⇓-lam : ∀{Γ}{γ : ClosEnv Γ}{M : Γ , ★ ⊢ ★}
        → γ ⊢ ƛ M ⇓ clos (ƛ M) γ

  ⇓-app : ∀{Γ}{γ : ClosEnv Γ}{L M : Γ ⊢ ★}{Δ}{δ : ClosEnv Δ}{N : Δ , ★ ⊢ ★}{c}
       → γ ⊢ L ⇓ clos (ƛ N) δ   →   (δ ,' clos M γ) ⊢ N ⇓ c
         ----------------------------------------------------
       → γ ⊢ L · M ⇓ c
\end{code}

* The `⇓-var` rule evaluates a variable by finding the associated
  closure in the environment and then evaluating the closure.

* The `⇓-lam` rule turns a lambda abstraction into a closure
  by packaging it up with its environment.

* The `⇓-app` rule performs function application by first evaluating
  the term `L` in operator position. If that produces a closure containing
  a lambda abstraction `ƛ N`, then we evaluate the body `N` in an
  environment extended with the argument `M`. Note that `M` is not
  evaluated in rule `⇓-app` because this is call-by-name and not
  call-by-value.

If the call-by-name relation evaluates a term `M` to both `c` and
`c'`, then `c` and `c'` are identical. In other words, the big-step
relation is a partial function.

\begin{code}
⇓-determ : ∀{Γ}{γ : ClosEnv Γ}{M : Γ ⊢ ★}{c c' : Clos}
         → γ ⊢ M ⇓ c → γ ⊢ M ⇓ c'
         → c ≡ c'
⇓-determ (⇓-var eq1 mc) (⇓-var eq2 mc')
      with trans (sym eq1) eq2
... | refl = ⇓-determ mc mc'
⇓-determ ⇓-lam ⇓-lam = refl
⇓-determ (⇓-app mc mc₁) (⇓-app mc' mc'') 
    with ⇓-determ mc mc'
... | refl = ⇓-determ mc₁ mc''
\end{code}

## A logical relation between call-by-name closures and terms

\begin{code}
𝔹 : Clos → (∅ ⊢ ★) → Set
ℍ : ∀{Γ} → ClosEnv Γ → Subst Γ ∅ → Set

𝔹 (clos {Γ} M γ) N = Σ[ σ ∈ Subst Γ ∅ ] ℍ γ σ × (N ≡ subst σ M)

ℍ γ σ = ∀{x} → 𝔹 (γ x) (σ x)
\end{code}

\begin{code}
ext-subst : ∀{Γ Δ} → Subst Γ Δ → Δ ⊢ ★ → Subst (Γ , ★) Δ
ext-subst{Γ}{Δ} σ N {A} = (subst (subst-zero N)) ∘ (exts σ)
\end{code}

\begin{code}
H-id : ℍ ∅' ids
H-id {()}
\end{code}

\begin{code}
ℍ-ext : ∀ {Γ} {γ : ClosEnv Γ} {σ : Subst Γ ∅} {c} {N : ∅ ⊢ ★}
      → ℍ γ σ  →  𝔹 c N
        --------------------------------
      → ℍ (γ ,' c) ((subst (subst-zero N)) ∘ (exts σ))
ℍ-ext {Γ} {γ} {σ} g e {Z} = e
ℍ-ext {Γ} {γ} {σ}{c}{N} g e {S x} = G g
  where
      eq : ext-subst σ N (S x) ≡ σ x
      eq =
        begin
          (subst (subst-zero N)) (exts σ (S x))
        ≡⟨⟩
          ((subst (subst-zero N)) ∘ (rename S_)) (σ x)
        ≡⟨ rename-subst{M = σ x} ⟩
          (subst ((subst-zero N) ∘ S_)) (σ x)        
        ≡⟨ sub-id ⟩
          σ x
        ∎
      G : 𝔹 (γ x) (σ x) → 𝔹 (γ x) (ext-subst σ N (S x))
      G b rewrite eq = b
\end{code}

\begin{code}
cbn→reduce : ∀{Γ}{γ : ClosEnv Γ}{σ : Subst Γ ∅}{M : Γ ⊢ ★}{c : Clos}
              → γ ⊢ M ⇓ c → ℍ γ σ
              → Σ[ N ∈ ∅ ⊢ ★ ] (subst σ M —↠ N) × 𝔹 c N
cbn→reduce {γ = γ} (⇓-var{x = x} eq d) h
    with γ x | h {x} | eq
... | clos M' γ' | ⟨ σ' , ⟨ h' , r ⟩ ⟩ | refl
    with cbn→reduce{σ = σ'} d h'
... | ⟨ N , ⟨ r' , bn ⟩ ⟩ rewrite r =    
      ⟨ N , ⟨ r' , bn ⟩ ⟩
cbn→reduce {Γ} {γ} {σ} {.(ƛ _)} {.(clos (ƛ _) γ)} (⇓-lam{M = N}) h =
   ⟨ subst σ (ƛ N) , ⟨ subst σ (ƛ N) [] , ⟨ σ , ⟨ h , refl ⟩ ⟩ ⟩ ⟩
cbn→reduce {Γ} {γ} {σ} {.(_ · _)} {c}
    (⇓-app{L = L}{M = M}{Δ = Δ}{δ = δ}{N = N} d₁ d₂) h
    with cbn→reduce{σ = σ} d₁ h
... | ⟨ L' , ⟨ σL—↠L' , ⟨ σ₁ , ⟨ Hδσ₁ , eq ⟩ ⟩ ⟩ ⟩ rewrite eq
    with cbn→reduce{σ = ext-subst σ₁ (subst σ M)} d₂
           (λ {x} → ℍ-ext{Δ}{σ = σ₁} Hδσ₁ (⟨ σ , ⟨ h , refl ⟩ ⟩){x})
       | β{∅}{subst (exts σ₁) N}{subst σ M}
... | ⟨ N' , ⟨ r' , bl ⟩ ⟩ | r 
    rewrite sub-sub{M = N}{σ₁ = exts σ₁}{σ₂ = subst-zero (subst σ M)} =
    let rs = (ƛ subst (exts σ₁) N) · subst σ M —→⟨ r ⟩ r' in
    ⟨ N' , ⟨ —↠-trans (appL-cong σL—↠L') rs , bl ⟩ ⟩
\end{code}

[JGS: to do: package up the above lemma into a nicer theorem]

[JGS: to do: forward reference the other direction of the proof in the
chapter on adequacy]
